"case TODO" on "Axiom TODO: False." prints what was "proved" using the axiom in "Print Assumptions end2endDemo."

bedrock2/src/Examples/Trace.v
@@ -167,7 +167,7 @@ Module SpiEth.
     (* TODO make coercions work *)
     (* Set Printing Implicit. Unset Printing Notations. *)
 
-    Definition TODO{T: Type}: T. Admitted.
+    Axiom TODO: False.
 
     Instance MMIOMacros: IOMacros.Interface := {|
       IOMacros.semantics_params := semantics_params;
@@ -195,7 +195,7 @@ Module SpiEth.
       eapply exec.seq with
           (mid := fun t' m' l' => t' = t /\ m' = m /\ l' = map.put l x (word.of_Z (-1))).
       { eapply exec.set; [reflexivity|auto]. }
-      { intros. apply TODO. (* will require a loop invariant *) }
+      { intros. case TODO. (* will require a loop invariant *) }
     - (* write_word_correct: *)
       intros.
       (* need to show that this imperative code corresponds to the Inductive write_byte *)
@@ -209,10 +209,10 @@ Module SpiEth.
             apply H.
             unfold isMMIOAddr.
             auto.
-          + apply TODO.
-        - apply TODO.
+          + case TODO.
+        - case TODO.
       }
-      apply TODO.
+      case TODO.
       Grab Existential Variables. all: intros; apply True.
     Defined.
 
@@ -282,7 +282,7 @@ Module Syscalls.
     (* TODO make coercions work *)
     (* Set Printing Implicit. Unset Printing Notations. *)
 
-    Definition TODO{T: Type}: T. Admitted.
+    Axiom TODO: False.
 
     Instance SyscallIOMacros: IOMacros.Interface := {|
       IOMacros.semantics_params := semantics_params;
@@ -313,10 +313,10 @@ Module Syscalls.
         eexists. repeat split.
         do 2 eexists. repeat split.
         * (* TODO direction doesn't match *)
-          apply TODO.
+          case TODO.
         * (* TODO need to specify that some ignored1, ignored2 are updated too *)
-          apply TODO.
-    - apply TODO.
+          case TODO.
+    - case TODO.
       Grab Existential Variables. all: apply (word.of_Z 42) || apply map.empty.
     Defined.
 
